example_loop_max.thy
@@ -126,6 +126,14 @@ definition inv :: "(proc, operation, val) invariantContext \<Rightarrow> bool" w
 
 definition "crdtSpec c op r = False"
 
+definition "crdtSpec' op Cs Ops  Hb C_out r = False"
+
+lemma crdtSpec_rel: 
+  shows "crdt_spec_rel crdtSpec crdtSpec'"
+  by (rule show_crdt_spec_rel')
+   (auto simp add: crdtSpec_def crdtSpec'_def)
+
+
 definition progr :: "(proc, localState, operation, val) prog" where
   "progr \<equiv> \<lparr>
   querySpec = crdtSpec,
@@ -224,9 +232,11 @@ proof M_show_programCorrect
           from `invariant_all' S`
           show "invariant_all' S" .
 
+          show "crdt_spec_rel (querySpec progr) crdtSpec'"
+            using crdtSpec_rel progr_def by simp
 
 
-          show "program_proof_rules_loops.execution_s_check (invariant progr) (querySpec progr) \<lparr>
+          show "program_proof_rules_loops.execution_s_check (invariant progr) crdtSpec' \<lparr>
                   calls = s_calls, 
                   happensBefore = s_happensBefore, 
                   callOrigin = s_callOrigin, 
